capsule-ltl/rust/aeneas/lean/lakefile.lean
@@ -1,8 +1,13 @@
 import Lake
 open Lake DSL
 
-require aeneas from "../aeneas-lean-lib"
+require aeneas from git
+  "https://github.com/AeneasVerif/aeneas.git" @
+  "45061fa1a5b4bad876f17c03d3a5544d818622e6" / "backends/lean"
+require papers4 from "../../../lean"
 
 package «capsulecheck» {}
 
-@[default_target] lean_lib «Capsule» {}
+@[default_target] lean_lib «Capsule» where
+  roots := #[`Capsule, `Authvar, `Secureboot, `AbstractAV, `AbstractSB,
+             `Bridge, `BridgeAV, `BridgeSB]
